Playing with false_elim and arrows with wps

rupicola/refinements/Compiler.fst
@@ -145,26 +145,7 @@ let test2_var : compile_exp (extend tunit (extend tunit empty)) (fun _ -> True) 
 let test3_var : compile_exp (extend tunit (extend tunit (extend tunit empty))) (fun _ -> True) (fun fs_s -> get_v' (fs_shrink (fs_shrink fs_s)) 0 unit) =
   solve
 
-
-(**
-instance compile_exp_lambda
-  g
-  (a:Type) {| ca: compile_typ a |}
-  (b:Type) {| cb: compile_typ b |}
-  (f:fs_env g -> a -> b)
-  {| cf: compile_exp #b #cb (extend (pack ca) g) (fun fs_s -> f (fs_shrink #(pack ca) fs_s) (get_v' fs_s 0 a)) |}
-  : compile_exp #_ #(compile_typ_arrow a b #ca #cb) g f = {
-  e = begin
-    lem_fv_in_env_lam g (pack ca) cf.e;
-    ELam cf.e
-  end;
-  equiv_proof = (fun () ->
-    cf.equiv_proof ();
-    reveal_opaque (`%get_v') (get_v' #(extend (pack ca) g));
-    equiv_lam g (pack ca) cf.e (pack cb) f;
-    assert (f `equiv (mk_arrow (pack ca) (pack cb))` (ELam cf.e))
-  )
-}**)
+(*** Compiling lambdas **)
 
 let get_body_f #g (pre:gpre g) a (#ca:compile_typ a) b (#cb:compile_typ b) wp (f:fs_oexp pre (x:a -> PURE b (wp x)))
   : fs_oexp #(extend (pack ca) g) (mk_pre_lam pre #(pack ca) #(pack cb) wp) b =
@@ -285,25 +266,27 @@ let test1_hoc : compile_closed
       (fun fs_s -> get_v' fs_s 0 _) #solve
       (fun _ -> false) #solve
       ())
+ **)
 
 instance compile_exp_if
   g
-  (co:fs_env g -> bool)  {| cco: compile_exp #_ #solve g co |}
+  gpre
+  (co:fs_oexp gpre bool)  {| cco: compile_exp g gpre co |}
 
   (#a:Type) {| ca: compile_typ a |}
-  (th:fs_env g -> a)     {| cth: compile_exp #_ #ca g th |}
-  (el:fs_env g -> a)     {| cel: compile_exp #_ #ca g el |}
-  : compile_exp #_ #ca g (fun fs_s -> if co fs_s then th fs_s else el fs_s) = {
+  (th:fs_oexp gpre a)     {| cth: compile_exp #_ #ca g gpre th |}
+  (el:fs_oexp gpre a)     {| cel: compile_exp #_ #ca g gpre el |}
+  : compile_exp #_ #ca g gpre (fun fs_s -> if co fs_s then th fs_s else el fs_s) = {
   e = begin
     lem_fv_in_env_if g cco.e cth.e cel.e;
     EIf cco.e cth.e cel.e
   end;
-  equiv_proof = (fun () ->
-    cco.equiv_proof ();
+  equiv_proof = (fun () -> admit ());
+ (**   cco.equiv_proof ();
     cth.equiv_proof ();
     cel.equiv_proof ();
     equiv_if g (pack ca) cco.e cth.e cel.e co th el
-  );
+  );**)
 }
 
 
@@ -315,19 +298,20 @@ let myt = true
 let test2_if : compile_closed #bool (if myt then false else true) = solve
 let _ = assert (test2_if.e == EIf ETrue EFalse ETrue)
 
+(**
 let test1_hoc : compile_closed
   #((bool -> bool) -> bool)
   #(compile_typ_arrow _ _ #(compile_typ_arrow _ _ #compile_typ_bool #compile_typ_bool))
   (fun f -> f false) =
-  compile_exp_lambda _ _ _ _ #(compile_exp_app _ _ _ (fun fs_s -> get_v' fs_s 0 (bool -> bool)) _)
+  compile_exp_lambda _ _ _ _ #(compile_exp_app _ _ _ (fun fs_s -> get_v' fs_s 0 (bool -> bool)) _)**)
 
 instance compile_exp_refinement
-  g
+  g gpre
   (#a:Type) {| ca: compile_typ a |}
   (p:a -> Type0)
-  (v:fs_env g -> (x:a{p x}))
-  {| cv: compile_exp #a #solve g v |}
-  : compile_exp #(x:a{p x}) #solve g (fun fs_s -> v fs_s) = {
+  (v:fs_oexp gpre (x:a{p x}))
+  {| cv: compile_exp #a #ca g (fun fs_s -> gpre fs_s /\ p (v fs_s)) v |} (** CA: Insane! I was throwing the refinement. I have to push it inside **)
+  : compile_exp #(x:a{p x}) #solve g gpre v = {
   e = cv.e;
   equiv_proof = (fun () ->
     cv.equiv_proof ()
@@ -344,8 +328,9 @@ let test2_ref : compile_closed (fun (x:bool{x == true}) -> x) =
   solve
 let _ = assert (test2_ref.e == ELam (EVar 0))
 
-let test3_ref : compile_closed (fun (x y:bool{False}) -> y) =
-  solve
+(**
+val test3_ref : compile_closed (fun (x y:bool{False}) -> y)
+let test3_ref = solve
 
 let test3_ref' : compile_closed (fun (x y:bool{False}) -> x) =
   solve
@@ -367,11 +352,9 @@ let _ = assert (test3_ref.e == ELam (ELam (EVar 0)))
 
    Which means that for test2 it quantifies over singleton true,
    and for test3 it quantifies over nothing.
-
-   I suppose now there is the question: how do we fix the interface
-   so that something this weird cannot happen?
 **)
 
+**)
 
 let test7_ref : compile_closed #(x:bool -> y:bool{y == false}) (fun x -> if x then false else false) =
   solve
@@ -387,18 +370,74 @@ let _ = assert (test_ref_assume'.e == ELam (EVar 0))
 let test_pm2 : (x:bool -> y:bool{y == false}) = (fun x -> if x then if x then false else true else false)
 let test_pm2' : compile_closed test_pm2 = solve
 let _ = assert (test_pm2'.e == ELam (EIf (EVar 0) (EIf (EVar 0) EFalse ETrue) EFalse))
-  (** why does this work? how did it type `true` to `y:bool{y == false}`?
 
-      My intuition says that it should fail
-      because the else branch, `fun _ -> true` has to be typed as `fs_env g -> y:bool{y == false}`,
-      which should fail because it tries to do it without knowing that `x == false`, which would produce a
-      contradiction with the initial refinement `x == true`.
-  **)
+
+instance compile_exp_false_elim
+  g pre
+  (a:Type) {| ca: compile_typ a |}
+  : compile_exp g pre (fun _ -> false_elim #a) = {
+  e = ELam EUnit;
+  equiv_proof = (fun () -> admit ()); (** this should be pretty easy to prove **)
+}
+
+(**
+instance compile_exp_refinement_intro
+  g pre
+  (#a:Type) {| ca: compile_typ a |}
+  (p:a -> Type0)
+  (v:fs_oexp pre a)
+  (l:(squash (forall fs_s. pre fs_s ==> p (v fs_s))))
+  {| cv: compile_exp #a #ca g pre v |}
+  : compile_exp #(x:a{p x}) #solve g pre (fun fs_s -> v fs_s) = {
+  e = cv.e;
+  equiv_proof = (fun () ->
+    cv.equiv_proof ()
+  );
+}*)
+
+let test_pm_false_elim0 : (x:unit -> Pure bool (requires False) (ensures fun _ -> True)) = (fun x -> false_elim ())
+let test_pm_false_elim0' : compile_closed test_pm_false_elim0 =
+ compile_exp_lambda_wp _ _ _ _ _ _
+   #(compile_exp_app _ _ _ _ _ _ #(compile_exp_false_elim _ _ _) _ _)
+
+(**
+ compile_exp_lambda_wp empty
+   (fun _ -> l_True)
+   unit
+   #compile_typ_unit
+   bool
+   #compile_typ_bool
+   (fun _ p -> l_False /\ (forall (pure_result: bool). l_True ==> p pure_result))
+   (fun _ -> test_pm_false_elim0)
+   #(compile_exp_app
+     (extend (pack #unit compile_typ_unit) empty)
+     (mk_pre_lam #empty
+         (fun _ -> l_True)
+         #(pack #unit compile_typ_unit)
+         #(pack #bool compile_typ_bool)
+         (fun _ p -> l_False /\ (forall (pure_result: bool). l_True ==> p pure_result)))
+     _
+     _
+     _
+     _ #(compile_exp_false_elim _ _ _)
+     (fun _ -> ()) #(compile_exp_refinement_intro _ _ _ _ ())
+     ())
+**)
+
+let test_pm_false_elim1 : (x:unit{False} -> Tot bool) = (fun x -> false_elim ())
+let test_pm_false_elim1' : compile_closed test_pm_false_elim1 =
+ compile_exp_lambda_wp _ _ _ _ _ _
+   #(compile_exp_app _ _ _ _ _ _ #(compile_exp_false_elim _ _ _) _ _)
+
+(**
+let test_pm_false_elim : (bool -> bool) = (fun x -> if x then if x then false else false_elim () else false)
+let test_pm_false_elim' : compile_closed test_pm_false_elim = solve
+**)
 
 let test_ref_precond_f (x:bool{x == true}) : bool = false
 let test_ref_precond : compile_closed #(bool -> bool) (fun x -> test_ref_precond_f (test_ref_assume x)) =
   solve
-let _ = assert (test_ref_precond.e == ELam EFalse) by (compute (); dump "H")
+let _ = assert (test_ref_precond.e == ELam EFalse)
 
 let test_ref_erasure (x:bool{x == true}) : bool = x
 
@@ -406,13 +445,13 @@ val test_ref_erasure' : compile_closed test_ref_erasure
 [@expect_failure]
 let test_ref_erasure' = solve (** this fails **)
 
-instance compile_exp_erase_refinement
-  g
+instance compile_exp_refinement_elim
+  g pre
   (a:Type) {| ca: compile_typ a |}
   (p:a -> Type0)
-  (v:fs_env g -> (x:a{p x}))
-  {| cv: compile_exp #(x:a{p x}) #(compile_typ_refinement a #ca p) g v |}
-  : compile_exp #a #ca g v = {
+  (v:fs_oexp pre (x:a{p x}))
+  {| cv: compile_exp #(x:a{p x}) #(compile_typ_refinement a #ca p) g pre v |}
+  : compile_exp #a #ca g pre v = {
   e = cv.e;
   equiv_proof = (fun () ->
     cv.equiv_proof ()
@@ -420,9 +459,9 @@ instance compile_exp_erase_refinement
 }
 
 let test_ref_erasure' =
-  compile_exp_lambda _ _ _ _
-    #(compile_exp_erase_refinement
-      _ _
+  compile_exp_lambda_wp _ _ _ _ _ _
+    #(compile_exp_refinement_elim
+      _ _ _
       (fun x -> x == true)
       (fun fs -> get_v' fs 0 (x:bool{x == true})))
 
@@ -431,8 +470,6 @@ let _ = assert (test_ref_erasure'.e == ELam (EVar 0))
 let test_pm1 : (x:bool{x == true} -> bool) = (fun x -> if x then false else true)
 [@expect_failure]
 let test_pm1' : compile_closed test_pm1 = solve (** I suppose this would work if test_ref_erasure works **)
-
-
 
 (**
 instance compile_exp_subtype
@@ -482,4 +519,3 @@ let test3_lem () : Lemma (True) = ()
 let test3_phase1 : compile_closed #(unit -> unit) (fun _ -> test3_lem ()) =
   solve
 let _ = assert (test3_phase1.e == ELam EUnit)
-**)
